deps/poulet4/lib/P4light/Architecture/Tofino.v
@@ -403,6 +403,9 @@ Definition extern_get_entries (es : extern_state) (p : path) : list table_entry 
   | _ => nil
   end.
 
+Definition extern_set_entries (es : extern_state) (p : path) (entries : list table_entry) : extern_state :=
+  PathMap.set p (ObjTable entries) es.
+
 Definition check_lpm_count (mks: list ident): option nat :=
   match findi (String.eqb "lpm") mks with
   | None => Some (List.length mks)
@@ -603,6 +606,7 @@ Instance TofinoExternSem : ExternSem := Build_ExternSem
   interp_extern
   interp_extern_safe
   extern_get_entries
+  extern_set_entries
   extern_match.
 
 Inductive exec_prog : (path -> extern_state -> list Val -> extern_state -> list Val -> signal -> Prop) ->
